Zippy/Zippy/Seqs/Zippy_Seqs.thy
@@ -1,0 +1,10 @@
+\<^marker>\<open>creator "Kevin Kappelmann"\<close>
+theory Zippy_Seqs
+  imports
+    ML_Typeclasses.ML_State
+    ML_Morphs
+begin
+
+ML_file\<open>zippy_seq_from_monad_mixin_base.ML\<close>
+
+end
